typing/pure_typingScript.sml
@@ -379,7 +379,7 @@ Inductive type_cexp:
 [~Lam:]
   (EVERY (type_ok (SND ns) db) arg_tys ∧
    LENGTH arg_tys = LENGTH xs ∧ arg_tys ≠ [] ∧
-   type_cexp ns db st (ZIP (xs, MAP ($, 0) arg_tys) ++ env) e ret_ty
+   type_cexp ns db st (REVERSE (ZIP (xs, MAP ($, 0) arg_tys)) ++ env) e ret_ty
       ⇒ type_cexp ns db st env (Lam c xs e) (Function arg_tys ret_ty)) ∧
 
 [~Let:]
@@ -419,7 +419,7 @@ Inductive type_cexp:
           MAP (tsubst tyargs) schemes = ptys ∧
         (* Continuation is well-typed: *)
           type_cexp (exndef,typedefs) db st
-            (ZIP (pvars, MAP ($, 0) ptys) ++ (v,0,TypeCons tyid tyargs)::env)
+            (REVERSE (ZIP (pvars, MAP ($, 0) ptys)) ++ (v,0,TypeCons tyid tyargs)::env)
             cexp t
       ) css ⇒
       type_cexp (exndef,typedefs) db st env (Case c e v css) t)
